FOmegaC/Agreement.v
@@ -1,0 +1,392 @@
+Require Import Coq.Lists.List.
+Require Export ParDB.Spec.
+Require Export ParDB.Lemmas.
+Require Export ParDB.Inst.
+
+Require Export SpecSyntax.
+Require Export SpecTyping.
+Require Export LemmasTyping.
+
+Local Ltac crush :=
+  intros;
+  repeat
+    (cbn in *;
+     (* repeat crushStlcSyntaxMatchH; *)
+     repeat crushDbSyntaxMatchH;
+     repeat crushDbLemmasRewriteH;
+     repeat crushSyntaxRefold;
+     repeat crushTypingMatchH;
+     subst*;
+     try discriminate;
+     eauto 200 with ws;
+     idtac
+    ).
+
+Lemma red_co {Γ γ σ τ k} :
+  ⟨ Γ ⊢ γ : σ ↝ τ ∷ k ⟩ →
+  ⟨ Γ ⊢ γ : σ ~ τ ∷ k ⟩.
+Proof. induction 1; eauto using Co, Ty. Qed.
+Hint Resolve red_co : ws.
+
+Definition cofromredstar (σ: Exp) (γs: list Exp) : Exp :=
+  fold_right (fun γ2 γ1 => cotrans γ1 γ2) (corefl σ) γs.
+
+Lemma redstar_co {Γ γs σ τ k} :
+  ⟨ Γ ⊢ γs : σ ↝* τ ∷ k ⟩ →
+  ⟨ Γ ⊢ cofromredstar σ γs : σ ~ τ ∷ k ⟩.
+Proof. induction 1; crush. Qed.
+Hint Resolve redstar_co : ws.
+
+Record WfEnv (Γ: Env) : Prop :=
+  { wfenv_covar_kind_left : ∀ c σ τ k, ⟨ c : σ ~ τ ∷ k ∈ Γ ⟩ → ⟨ Γ ⊢ σ ∷ k ⟩;
+    wfenv_covar_kind_right : ∀ c σ τ k, ⟨ c : σ ~ τ ∷ k ∈ Γ ⟩ → ⟨ Γ ⊢ τ ∷ k ⟩
+  }.
+Hint Resolve wfenv_covar_kind_left.
+Hint Resolve wfenv_covar_kind_right.
+
+Lemma wfenv_snoc_tyvar {Γ} (wΓ: WfEnv Γ) : ∀ k, WfEnv (Γ ► k).
+Proof. constructor; crush; eauto with ws. Qed.
+Hint Resolve wfenv_snoc_tyvar : ws.
+
+Lemma co_agreement {Γ γ σ τ k} (wΓ: WfEnv Γ) (wγ: ⟨ Γ ⊢ γ : σ ~ τ ∷ k ⟩) :
+  ⟨ Γ ⊢ σ ∷ k ⟩ ∧ ⟨ Γ ⊢ τ ∷ k ⟩.
+Proof.
+  induction wγ; intuition; crush;
+  match goal with
+    | [IH: WfEnv (?Γ ► ?k) → _ |- _] =>
+      enough (WfEnv (Γ ► k)); intuition; crush
+  end.
+Qed.
+
+Lemma co_agreement_left {Γ γ σ τ k} (wΓ: WfEnv Γ) (wγ: ⟨ Γ ⊢ γ : σ ~ τ ∷ k ⟩) :
+  ⟨ Γ ⊢ σ ∷ k ⟩.
+Proof. eapply co_agreement; eauto with ws. Qed.
+Hint Resolve co_agreement_left : ws.
+
+Lemma co_agreement_right {Γ γ σ τ k} (wΓ: WfEnv Γ) (wγ: ⟨ Γ ⊢ γ : σ ~ τ ∷ k ⟩) :
+  ⟨ Γ ⊢ τ ∷ k ⟩.
+Proof. eapply co_agreement; eauto with ws. Qed.
+Hint Resolve co_agreement_right : ws.
+
+(******************************************************************************)
+
+Fixpoint redrefl (τ: Exp) : Exp :=
+  match τ with
+    | var α           => corefl (var α)
+    | τabs k τ        => coτabs k (redrefl τ)
+    | τapp τ1 τ2      => coτapp (redrefl τ1) (redrefl τ2)
+    | arr τ1 τ2       => coarr (redrefl τ1) (redrefl τ2)
+    | arrτ k τ        => coarrτ k (redrefl τ)
+    | arrγ τ1 τ2 k τ3 => coarrγ (redrefl τ1) (redrefl τ2) k (redrefl τ3)
+    | _ => var 0
+  end.
+
+Lemma RedRefl {Γ τ k} (wτ: ⟨ Γ ⊢ τ ∷ k ⟩) :
+  ⟨ Γ ⊢ redrefl τ : τ ↝ τ ∷ k ⟩.
+Proof. induction wτ; crush. Qed.
+Hint Resolve RedRefl : ws.
+
+
+Definition rstrans (γs1 γs2: list Exp) : list Exp :=
+  List.app γs2 γs1.
+Lemma RsTrans {Γ γs1 γs2 τ1 τ2 τ3 k} :
+  ⟨ Γ ⊢ γs1 : τ1 ↝* τ2 ∷ k ⟩ →
+  ⟨ Γ ⊢ γs2 : τ2 ↝* τ3 ∷ k ⟩ →
+  ⟨ Γ ⊢ rstrans γs1 γs2 : τ1 ↝* τ3 ∷ k ⟩.
+Proof. intros wγs1 wγs2; induction wγs2; crush. Qed.
+
+
+Definition rsτabs (k: Kind) (γs: list Exp) : list Exp :=
+  List.map (coτabs k) γs.
+Lemma RsTAbs {Γ γs σ τ k1 k2} :
+  ⟨ Γ ► k1 ⊢ γs : σ ↝* τ ∷ k2 ⟩ →
+  ⟨ Γ ⊢ rsτabs k1 γs : τabs k1 σ ↝* τabs k1 τ ∷ karr k1 k2 ⟩.
+Proof. intros wγs; depind wγs; crush. Qed.
+
+
+Definition rsτapp₁ (γs: list Exp) (τ: Exp) : list Exp :=
+  List.map (fun γ => coτapp γ (redrefl τ)) γs.
+Definition rsτapp₂ (σ: Exp) (γs: list Exp)  : list Exp :=
+  List.map (coτapp (redrefl σ)) γs.
+Definition rsτapp (σγs: list Exp) (σ1 σ2: Exp) (τγs: list Exp) (τ1 τ2 : Exp) : list Exp :=
+  rstrans (rsτapp₁ σγs τ1) (rsτapp₂ σ2 τγs).
+
+Lemma RsTApp₁ {Γ γs σ1 σ2 τ k1 k2} :
+  ⟨ Γ ⊢ γs : σ1 ↝* σ2 ∷ karr k1 k2 ⟩ →
+  ⟨ Γ ⊢ τ ∷ k1 ⟩ →
+  ⟨ Γ ⊢ rsτapp₁ γs τ : τapp σ1 τ ↝* τapp σ2 τ ∷ k2 ⟩.
+Proof. intros wγs wτ; unfold rsτapp₁; depind wγs; crush. Qed.
+Lemma RsTApp₂ {Γ γs τ1 τ2 σ k1 k2} :
+  ⟨ Γ ⊢ σ ∷ karr k1 k2 ⟩ →
+  ⟨ Γ ⊢ γs : τ1 ↝* τ2 ∷ k1 ⟩ →
+  ⟨ Γ ⊢ rsτapp₂ σ γs: τapp σ τ1 ↝* τapp σ τ2 ∷ k2 ⟩.
+Proof. intros wσ wγs; unfold rsτapp₂; depind wγs; crush. Qed.
+
+Lemma RsTApp {Γ σγs τγs σ1 σ2 τ1 τ2 k1 k2} :
+  ⟨ Γ ⊢ σ2 ∷ karr k1 k2 ⟩ →
+  ⟨ Γ ⊢ σγs : σ1 ↝* σ2 ∷ karr k1 k2 ⟩ →
+  ⟨ Γ ⊢ τ1 ∷ k1 ⟩ →
+  ⟨ Γ ⊢ τγs : τ1 ↝* τ2 ∷ k1 ⟩ →
+  ⟨ Γ ⊢ rsτapp σγs σ1 σ2 τγs τ1 τ2 : τapp σ1 τ1 ↝* τapp σ2 τ2 ∷ k2 ⟩.
+Proof.
+  intros.
+  eapply RsTrans.
+  - eapply RsTApp₁; crush.
+  - eapply RsTApp₂; crush.
+Qed.
+
+
+Definition rsarr₁ (γs: list Exp) (τ: Exp) : list Exp :=
+  List.map (fun γ => coarr γ (redrefl τ)) γs.
+Definition rsarr₂ (σ: Exp) (γs: list Exp)  : list Exp :=
+  List.map (coarr (redrefl σ)) γs.
+Definition rsarr (σγs: list Exp) (σ1 σ2: Exp) (τγs: list Exp) (τ1 τ2 : Exp) : list Exp :=
+  rstrans (rsarr₁ σγs τ1) (rsarr₂ σ2 τγs).
+
+Lemma RsArr₁ {Γ σγs σ1 σ2 τ} :
+  ⟨ Γ ⊢ σγs : σ1 ↝* σ2 ∷ kstar ⟩ →
+  ⟨ Γ ⊢ τ ∷ kstar ⟩ →
+  ⟨ Γ ⊢ rsarr₁ σγs τ : arr σ1 τ ↝* arr σ2 τ ∷ kstar ⟩.
+Proof. intros wσγs wτ; unfold rsarr₁; depind wσγs; crush. Qed.
+Lemma RsArr₂ {Γ σ τγs τ1 τ2} :
+  ⟨ Γ ⊢ σ ∷ kstar ⟩ →
+  ⟨ Γ ⊢ τγs : τ1 ↝* τ2 ∷ kstar ⟩ →
+  ⟨ Γ ⊢ rsarr₂ σ τγs: arr σ τ1 ↝* arr σ τ2 ∷ kstar ⟩.
+Proof. intros wσ wτγs; unfold rsarr₂; depind wτγs; crush. Qed.
+
+Lemma RsArr {Γ σγs σ1 σ2 τγs τ1 τ2} :
+  ⟨ Γ ⊢ σ2 ∷ kstar ⟩ →
+  ⟨ Γ ⊢ σγs : σ1 ↝* σ2 ∷ kstar ⟩ →
+  ⟨ Γ ⊢ τ1 ∷ kstar ⟩ →
+  ⟨ Γ ⊢ τγs : τ1 ↝* τ2 ∷ kstar ⟩ →
+  ⟨ Γ ⊢ rsarr σγs σ1 σ2 τγs τ1 τ2 : arr σ1 τ1 ↝* arr σ2 τ2 ∷ kstar ⟩.
+Proof.
+  intros.
+  eapply RsTrans.
+  - eapply RsArr₁; crush.
+  - eapply RsArr₂; crush.
+Qed.
+
+
+Definition rsarrτ (k: Kind) (γs: list Exp) : list Exp :=
+  List.map (coarrτ k) γs.
+Lemma RsArrT {Γ γs σ τ k} :
+  ⟨ Γ ► k ⊢ γs : σ ↝* τ ∷ kstar ⟩ →
+  ⟨ Γ ⊢ rsarrτ k γs : arrτ k σ ↝* arrτ k τ ∷ kstar ⟩.
+Proof. intros wγs; depind wγs; crush. Qed.
+
+
+Definition rsarrγ₁ (σγs: list Exp) (τ: Exp) (k: Kind) (ν: Exp) : list Exp :=
+  List.map (fun σγ => coarrγ σγ (redrefl τ) k (redrefl ν)) σγs.
+Definition rsarrγ₂ (σ: Exp) (τγs: list Exp) (k: Kind) (ν: Exp) : list Exp :=
+  List.map (fun τγ => coarrγ (redrefl σ) τγ k (redrefl ν)) τγs.
+Definition rsarrγ₃ (σ: Exp) (τ: Exp) (k: Kind) (νγs: list Exp) : list Exp :=
+  List.map (fun νγ => coarrγ (redrefl σ) (redrefl τ) k νγ) νγs.
+Definition rsarrγ (σγs: list Exp) (σ σ': Exp) (τγs: list Exp) (τ τ': Exp) k (νγs: list Exp) (ν ν': Exp) : list Exp :=
+  rstrans (rsarrγ₁ σγs τ k ν) (rstrans (rsarrγ₂ σ' τγs k ν) (rsarrγ₃ σ' τ' k νγs)).
+
+Lemma RsArrG₁ {Γ σγs σ σ' τ k ν} :
+  ⟨ Γ ⊢ σγs : σ ↝* σ' ∷ k ⟩ →
+  ⟨ Γ ⊢ τ ∷ k ⟩ →
+  ⟨ Γ ⊢ ν ∷ kstar ⟩ →
+  ⟨ Γ ⊢ rsarrγ₁ σγs τ k ν : arrγ σ τ k ν ↝* arrγ σ' τ k ν ∷ kstar ⟩.
+Proof. intros wσγs wτ wν; unfold rsarrγ₁; depind wσγs; crush. Qed.
+Lemma RsArrG₂ {Γ σ τγs τ τ' k ν} :
+  ⟨ Γ ⊢ σ ∷ k ⟩ →
+  ⟨ Γ ⊢ τγs : τ ↝* τ' ∷ k ⟩ →
+  ⟨ Γ ⊢ ν ∷ kstar ⟩ →
+  ⟨ Γ ⊢ rsarrγ₂ σ τγs k ν : arrγ σ τ k ν ↝* arrγ σ τ' k ν ∷ kstar ⟩.
+Proof. intros wσ wτγs wν; unfold rsarrγ₂; depind wτγs; crush. Qed.
+Lemma RsArrG₃ {Γ σ τ k νγs ν ν'} :
+  ⟨ Γ ⊢ σ ∷ k ⟩ →
+  ⟨ Γ ⊢ τ ∷ k ⟩ →
+  ⟨ Γ ⊢ νγs : ν ↝* ν' ∷ kstar ⟩ →
+  ⟨ Γ ⊢ rsarrγ₃ σ τ k νγs : arrγ σ τ k ν ↝* arrγ σ τ k ν' ∷ kstar ⟩.
+Proof. intros wσ wτ wνγs; unfold rsarrγ₃; depind wνγs; crush. Qed.
+
+Lemma RsArrG {Γ σγs σ σ' τγs τ τ' k νγs ν ν'} :
+  ⟨ Γ ⊢ σ' ∷ k ⟩ →
+  ⟨ Γ ⊢ σγs : σ ↝* σ' ∷ k ⟩ →
+  ⟨ Γ ⊢ τ ∷ k ⟩ →
+  ⟨ Γ ⊢ τ' ∷ k ⟩ →
+  ⟨ Γ ⊢ τγs : τ ↝* τ' ∷ k ⟩ →
+  ⟨ Γ ⊢ ν ∷ kstar ⟩ →
+  ⟨ Γ ⊢ νγs : ν ↝* ν' ∷ kstar ⟩ →
+  ⟨ Γ ⊢ rsarrγ σγs σ σ' τγs τ τ' k νγs ν ν' : arrγ σ τ k ν ↝* arrγ σ' τ' k ν' ∷ kstar ⟩.
+Proof.
+  intros.
+  eapply RsTrans.
+  eapply RsArrG₁; crush.
+  eapply RsTrans.
+  eapply RsArrG₂; crush.
+  eapply RsArrG₃; crush.
+Qed.
+
+
+Definition rsbeta (k: Kind) (σγs: list Exp) (σ σ': Exp) (τγs: list Exp) (τ τ': Exp) : list Exp :=
+  cons (cobeta k (redrefl σ') (redrefl τ')) (rsτapp (rsτabs k σγs) (τabs k σ) (τabs k σ') τγs τ τ').
+
+Lemma RsBeta {Γ σγs σ σ' τγs τ τ' k1 k2} :
+  ⟨ Γ ► k1 ⊢ σ' ∷ k2 ⟩ →
+  ⟨ Γ ► k1 ⊢ σγs : σ ↝* σ' ∷ k2 ⟩ →
+  ⟨ Γ ⊢ τ ∷ k1 ⟩ →
+  ⟨ Γ ⊢ τ' ∷ k1 ⟩ →
+  ⟨ Γ ⊢ τγs : τ ↝* τ' ∷ k1 ⟩ →
+  ⟨ Γ ⊢ rsbeta k1 σγs σ σ' τγs τ τ' : τapp (τabs k1 σ) τ ↝* σ'[beta1 τ'] ∷ k2 ⟩.
+Proof.
+  intros. unfold rsbeta.
+  econstructor.
+  - eapply RsTApp; eauto.
+    + constructor; auto.
+    + eapply RsTAbs; eauto.
+  - constructor; eauto.
+    + eapply RedRefl; eauto.
+    + eapply RedRefl; eauto.
+Qed.
+
+
+(* Definition coredstarbeta₁ (k: Kind) (γs: list Exp) (τ: Exp) : list Exp := *)
+(*   List.map (fun γ => cobeta k γ (redrefl τ)) γs. *)
+(* Lemma RedStarBeta₁ {Γ γsσ σ σ' γsτ τ τ' k1 k2} : *)
+(*   ⟨ Γ ► k1 ⊢ γsσ : σ ↝* σ' ∷ k2 ⟩ → *)
+(*   ⟨ Γ ⊢ γsτ : τ ~ τ' ∷ k1 ⟩ → *)
+(*   ∃ ηs, ⟨ Γ ⊢ ηs : τapp (τabs k1 σ) τ ↝* σ'[beta1 τ'] ∷ k2 ⟩. *)
+(* Proof.   *)
+(*   unfold coredstarbeta₁; depind rσ; crush. *)
+(* Qed. *)
+
+(* Definition coredstarbeta₂ (σ: Exp) (γs: list Exp)  : list Exp := *)
+(*   List.map (cobeta (redrefl σ)) γs. *)
+(* Lemma RedStarBeta₂ {Γ γs τ1 τ2} (rτ: ⟨ Γ ⊢ γs : τ1 ↝* τ2 ∷ kstar ⟩) : *)
+(*   ∀ {σ}, ⟨ Γ ⊢ σ ∷ kstar ⟩ → ⟨ Γ ⊢ coredstarbeta₂ σ γs: beta σ τ1 ↝* beta σ τ2 ∷ kstar ⟩. *)
+(* Proof. unfold coredstarbeta₂; depind rτ; crush. Qed. *)
+
+(* Definition coredstarbeta (σγs: list Exp) (σ1 σ2: Exp) (τγs: list Exp) (τ1 τ2 : Exp) : list Exp := *)
+(*   rstrans (coredstarbeta₁ σγs τ1) (coredstarbeta₂ σ2 τγs). *)
+(* Lemma RedStarBeta {Γ σγs τγs σ1 σ2 τ1 τ2} (wΓ: WfEnv Γ) *)
+(*   (wσγs: ⟨ Γ ⊢ σγs : σ1 ↝* σ2 ∷ kstar ⟩) *)
+(*   (wτγs: ⟨ Γ ⊢ τγs : τ1 ↝* τ2 ∷ kstar ⟩) : *)
+(*   ⟨ Γ ⊢ coredstarbeta σγs σ1 σ2 τγs τ1 τ2 : beta σ1 τ1 ↝* beta σ2 τ2 ∷ kstar ⟩. *)
+(* Proof. *)
+(*   eapply RsTrans. *)
+(*   - eapply RedStarBeta₁; crush. *)
+(*   - eapply RedStarBeta₂; crush. *)
+(* Qed. *)
+
+(*
+Definition rstrans (γs1 γs2: list Exp) : list Exp :=
+  List.app γs2 γs1.
+
+Lemma RsTrans {Γ γs1 γs2 τ1 τ2 ν k} :
+  ⟨ Γ ⊢ γs1 : τ1 ↝* τ2 ∷ k ⟩ →
+  ⟨ Γ ⊢ γs2 : τ2 ↝* ν ∷ k ⟩ →
+  ⟨ Γ ⊢ rstrans γs1 γs2 : τ1 ↝* τ3 ∷ k ⟩.
+Proof. intros r q; revert τ1 r; induction q; crush. Qed.
+
+Fixpoint redrefl (τ: Exp) : Exp :=
+  match τ with
+    | var α           => corefl (var α)
+    | τabs k τ        => coτabs k (redrefl τ)
+    | τapp τ1 τ2      => coτapp (redrefl τ1) (redrefl τ2)
+    | arr τ1 τ2       => coarr (redrefl τ1) (redrefl τ2)
+    | arrτ k τ        => coarrτ k (redrefl τ)
+    | arrγ τ1 τ2 k τ3 => coarrγ (redrefl τ1) (redrefl τ2) k (redrefl τ3)
+    | _ => var 0
+  end.
+
+Lemma RedRefl {Γ τ k} (wτ: ⟨ Γ ⊢ τ ∷ k ⟩) :
+  ⟨ Γ ⊢ redrefl τ : τ ↝ τ ∷ k ⟩.
+Proof. induction wτ; crush. Qed.
+Hint Resolve RedRefl : ws.
+
+Definition rsτapp₁ (γs: list Exp) (τ: Exp) : list Exp :=
+  List.map (fun γ => coτapp γ (redrefl τ)) γs.
+Lemma RsTApp₁ {Γ γs σ1 σ2 k1 k2} (rσ: ⟨ Γ ⊢ γs : σ1 ↝* σ2 ∷ karr k1 k2 ⟩) :
+  ∀ {τ}, ⟨ Γ ⊢ τ ∷ k1 ⟩ → ⟨ Γ ⊢ rsτapp₁ γs τ : τapp σ1 τ ↝* τapp σ2 τ ∷ k2 ⟩.
+Proof. unfold rsτapp₁; depind rσ; crush. Qed.
+Definition rsτapp₂ (σ: Exp) (γs: list Exp)  : list Exp :=
+  List.map (coτapp (redrefl σ)) γs.
+Lemma RsTApp₂ {Γ γs τ1 τ2 k1} (rτ: ⟨ Γ ⊢ γs : τ1 ↝* τ2 ∷ k1 ⟩) :
+  ∀ {σ k2}, ⟨ Γ ⊢ σ ∷ karr k1 k2 ⟩ → ⟨ Γ ⊢ rsτapp₂ σ γs: τapp σ τ1 ↝* τapp σ τ2 ∷ k2 ⟩.
+Proof. unfold rsτapp₂; depind rτ; crush. Qed.
+
+Definition rsτapp (σγs: list Exp) (σ1 σ2: Exp) (τγs: list Exp) (τ1 τ2 : Exp) : list Exp :=
+  rstrans (rsτapp₁ σγs τ1) (rsτapp₂ σ2 τγs).
+Lemma RsTApp {Γ σγs τγs σ1 σ2 τ1 τ2 k1 k2} (wΓ: WfEnv Γ)
+  (wσγs: ⟨ Γ ⊢ σγs : σ1 ↝* σ2 ∷ karr k1 k2 ⟩)
+  (wτγs: ⟨ Γ ⊢ τγs : τ1 ↝* τ2 ∷ k1 ⟩) :
+  ⟨ Γ ⊢ rsτapp σγs σ1 σ2 τγs τ1 τ2 : τapp σ1 τ1 ↝* τapp σ2 τ2 ∷ k2 ⟩.
+Proof.
+  eapply RsTrans.
+  - eapply RsTApp₁; crush.
+  - eapply RsTApp₂; crush.
+Qed.
+
+Definition rsτabs (k: Kind) (γs: list Exp) : list Exp :=
+  List.map (coτabs k) γs.
+Lemma RsTAbs {Γ γs σ τ k1 k2} :
+  ⟨ Γ ► k1 ⊢ γs : σ ↝* τ ∷ k2 ⟩ →
+  ⟨ Γ ⊢ rsτabs k1 γs : τabs k1 σ ↝* τabs k1 τ ∷ karr k1 k2 ⟩.
+Proof. intros wγs; depind wγs; crush. Qed.
+
+
+Definition rsarr₁ (γs: list Exp) (τ: Exp) : list Exp :=
+  List.map (fun γ => coarr γ (redrefl τ)) γs.
+Lemma RsArr₁ {Γ γs σ1 σ2} (rσ: ⟨ Γ ⊢ γs : σ1 ↝* σ2 ∷ kstar ⟩) :
+  ∀ {τ}, ⟨ Γ ⊢ τ ∷ kstar ⟩ → ⟨ Γ ⊢ rsarr₁ γs τ : arr σ1 τ ↝* arr σ2 τ ∷ kstar ⟩.
+Proof. unfold rsarr₁; depind rσ; crush. Qed.
+Definition rsarr₂ (σ: Exp) (γs: list Exp)  : list Exp :=
+  List.map (coarr (redrefl σ)) γs.
+Lemma RsArr₂ {Γ γs τ1 τ2} (rτ: ⟨ Γ ⊢ γs : τ1 ↝* τ2 ∷ kstar ⟩) :
+  ∀ {σ}, ⟨ Γ ⊢ σ ∷ kstar ⟩ → ⟨ Γ ⊢ rsarr₂ σ γs: arr σ τ1 ↝* arr σ τ2 ∷ kstar ⟩.
+Proof. unfold rsarr₂; depind rτ; crush. Qed.
+
+Definition rsarr (σγs: list Exp) (σ1 σ2: Exp) (τγs: list Exp) (τ1 τ2 : Exp) : list Exp :=
+  rstrans (rsarr₁ σγs τ1) (rsarr₂ σ2 τγs).
+Lemma RsArr {Γ σγs τγs σ1 σ2 τ1 τ2} (wΓ: WfEnv Γ)
+  (wσγs: ⟨ Γ ⊢ σγs : σ1 ↝* σ2 ∷ kstar ⟩)
+  (wτγs: ⟨ Γ ⊢ τγs : τ1 ↝* τ2 ∷ kstar ⟩) :
+  ⟨ Γ ⊢ rsarr σγs σ1 σ2 τγs τ1 τ2 : arr σ1 τ1 ↝* arr σ2 τ2 ∷ kstar ⟩.
+Proof.
+  eapply RsTrans.
+  - eapply RsArr₁; crush.
+  - eapply RsArr₂; crush.
+Qed.
+
+
+(* Definition rsarrτ (k: Kind) (γs: list Exp) : list Exp := *)
+(*   List.map (coarrτ k) γs. *)
+(* Lemma RsArrT {Γ γs σ τ k} : *)
+(*   ⟨ Γ ► k ⊢ γs : σ ↝* τ ∷ kstar ⟩ → *)
+(*   ⟨ Γ ⊢ rsarrτ k γs : arrτ k σ ↝* arrτ k τ ∷ kstar ⟩. *)
+(* Proof. intros wγs; depind wγs; crush. Qed. *)
+
+
+(* Definition coredstarbeta₁ (k: Kind) (γs: list Exp) (τ: Exp) : list Exp := *)
+(*   List.map (fun γ => cobeta k γ (redrefl τ)) γs. *)
+(* Lemma RedStarBeta₁ {Γ γsσ σ σ' γsτ τ τ' k1 k2} : *)
+(*   ⟨ Γ ► k1 ⊢ γsσ : σ ↝* σ' ∷ k2 ⟩ → *)
+(*   ⟨ Γ ⊢ γsτ : τ ~ τ' ∷ k1 ⟩ → *)
+(*   ∃ ηs, ⟨ Γ ⊢ ηs : τapp (τabs k1 σ) τ ↝* σ'[beta1 τ'] ∷ k2 ⟩. *)
+(* Proof.   *)
+(*   unfold coredstarbeta₁; depind rσ; crush. *)
+(* Qed. *)
+
+(* Definition coredstarbeta₂ (σ: Exp) (γs: list Exp)  : list Exp := *)
+(*   List.map (cobeta (redrefl σ)) γs. *)
+(* Lemma RedStarBeta₂ {Γ γs τ1 τ2} (rτ: ⟨ Γ ⊢ γs : τ1 ↝* τ2 ∷ kstar ⟩) : *)
+(*   ∀ {σ}, ⟨ Γ ⊢ σ ∷ kstar ⟩ → ⟨ Γ ⊢ coredstarbeta₂ σ γs: beta σ τ1 ↝* beta σ τ2 ∷ kstar ⟩. *)
+(* Proof. unfold coredstarbeta₂; depind rτ; crush. Qed. *)
+
+(* Definition coredstarbeta (σγs: list Exp) (σ1 σ2: Exp) (τγs: list Exp) (τ1 τ2 : Exp) : list Exp := *)
+(*   rstrans (coredstarbeta₁ σγs τ1) (coredstarbeta₂ σ2 τγs). *)
+(* Lemma RedStarBeta {Γ σγs τγs σ1 σ2 τ1 τ2} (wΓ: WfEnv Γ) *)
+(*   (wσγs: ⟨ Γ ⊢ σγs : σ1 ↝* σ2 ∷ kstar ⟩) *)
+(*   (wτγs: ⟨ Γ ⊢ τγs : τ1 ↝* τ2 ∷ kstar ⟩) : *)
+(*   ⟨ Γ ⊢ coredstarbeta σγs σ1 σ2 τγs τ1 τ2 : beta σ1 τ1 ↝* beta σ2 τ2 ∷ kstar ⟩. *)
+(* Proof. *)
+(*   eapply RsTrans. *)
+(*   - eapply RedStarBeta₁; crush. *)
+(*   - eapply RedStarBeta₂; crush. *)
+(* Qed. *)
+*)
